% -*- root: Main.tex -*-
\section{Essentials}
\subsection*{Matrix/Vector}
\begin{compactdesc}
	\item $A\cdot B = C \Leftrightarrow c_{ik}=\sum_{j=1}^{m} a_{ij} \cdot b_{jk}, c=\sum_{i} a_i b_i^\top$
	\item $A^\top\cdot B = C \Leftrightarrow c_{ik}=a_i^\top \cdot b_k$
	\item $z=Ax\Leftrightarrow z_i=\sum_k a_{ik} x_k$
	\item $z^\top = y^\top A \Leftrightarrow z_i = \sum_k a_{ki} y_k$
	\item $A\cdot B=(A B^{(1)}\hspace{1pt} AB^{(2)}\hspace{1pt} \dots)=(A^{[1]}B\hspace{3pt}A^{[2]}B\hspace{3pt}\dots)^\top$
	\item $\mathbf{Ker}(A)=\{x|Ax=0\}$, $\mathbf{Im}(A)=\{y|\exists x.Ax=y\}$
	\item $\mathbf{Rank}(A) := dim(\mathbf{Im}(A))$
	\item $\mathbf{Rank}(A\cdot B) \leq min(\mathbf{Rank}(A), \mathbf{Rank}(B))$
	\item $dim(A)=\mathbf{Rank}(A) + dim(\mathbf{Ker}(A))$
	\item[Tr:] $\mathbf{Tr}(A) := \sum_i a_{ii}$, $\mathbf{Tr}(rA+sB)=r\mathbf{Tr}(A)+s\mathbf{Tr}(B)$, $\mathbf{Tr}(ABC)=\mathbf{Tr}(CAB)=\mathbf{Tr}(BCA)$
	\item[Vec(A):] Column by col. forming a new vector
	\item[det(A)=0:] $\exists$ linear dependent cols/rows
	\item[det(A)!=0:] $A$ regular, $Ax=b$ has 1 sol., $\exists A^{-1}$, $im(A)=\mathbb{M}^n, ker(A)=0$, 0 is not EW of $A$
	\item[Orthogonal:] cols. orthonormal, $\mathbf{A}^{-1} = \mathbf{A}^\top$, $\mathbf{A} \mathbf{A}^\top = \mathbf{A}^\top \mathbf{A} = \mathbf{I}$, $\operatorname{det}(\mathbf{A}) \in \{+1, -1\}$, $\operatorname{det}(\mathbf{A}^\top \mathbf{A}) = 1$, $(t\cdot A)^{-1}=1/t\cdot A^{-1}$, $A, B: orth \implies A\cdot B: orth$, Preserves norm ($||Ax||=x$), inner prod., dist., angle, EWs are on unit circle, EVs are unitary
	\item[Positive semi-definite:] $\forall x, x^\top A x \geq 0$, $Tr(A)\geq 0$, $A^{-1}$ psd., $\exists B . A=BB^\top$ with $\mathbf{Rank}(A)=\mathbf{Rank}(B)$, $x^\top A x = 0 \Rightarrow A x = 0$ $X\in \mathbb{R}^{n,r}, n\leq r, rank(X)=n \Rightarrow XX^\top$ psd.
	\item[Itempot.:] $A^2 = A$, $I-A$ idp. and $A(I-A)=0$, $rank(A)=tr(A)$, $CD$ idp. $\Rightarrow$ $CD=DC$, $f(sI+tA)=(I-A)f(s)+A f(s+t)$
	\item[Pseudo-Inverse:] $A\cdot A^+\cdot A = A$
	\item[Inner Product:] $\langle \mathbf{x}, \mathbf{y} \rangle = \mathbf{x}^\top \mathbf{y} = \sum_{i=1}^{N} \mathbf{x}_i \mathbf{y}_i$.
	\begin{inparaitem}
		\item $\langle \mathbf{x} \pm \mathbf{y}, \mathbf{x} \pm \mathbf{y} \rangle = \langle \mathbf{x}, \mathbf{x} \rangle \pm 2 \langle \mathbf{x}, \mathbf{y} \rangle + \langle \mathbf{y}, \mathbf{y} \rangle$
		\item $\langle \mathbf{x}, \mathbf{y} + \mathbf{z} \rangle = \langle \mathbf{x}, \mathbf{y} \rangle + \langle \mathbf{x}, \mathbf{z} \rangle$
		\item $\langle \mathbf{x} + \mathbf{y}, \mathbf{z} \rangle = \langle \mathbf{x}, \mathbf{z} \rangle + \langle \mathbf{y}, \mathbf{z} \rangle$
		\item $\langle \mathbf{x}, \mathbf{y} \rangle = \|\mathbf{x}\|_2 \cdot \|\mathbf{y}\|_2 \cdot \cos(\theta)$
		\item If $\mathbf{y}$ is a unit vector then $\langle \mathbf{x}, \mathbf{y} \rangle$ projects $\mathbf{x}$ onto $\mathbf{y}$
	\end{inparaitem}
	\item[Outer Product:] $\mathbf{u} \mathbf{v}^\top$, $(\mathbf{u} \mathbf{v}^\top)_{i, j} = \mathbf{u}_i \mathbf{v}_j$
	\item[Transp. + Inv.:] $(\mathbf{A}^\top)^{-1} = (\mathbf{A}^{-1})^\top$
	\item[Orth. proj.:] $P_y(x)=y y^\top x / ||y||^2_2 = <x,y>y$
	\item[Proj. to orth. compl.:] $v-<u,v>u$
	\item[Householder-Refl.:] $H_u=I-2uu^\top$ sym.+orth.
	\item[Jacobian:] $D f(x)=(\frac{\partial f_i(x)}{\partial x_j})_{i=1..m, j=1..n} \in \mathbb{R}^{m\cdot n}$
\end{compactdesc}

\subsection*{Norms}
$\|\mathbf{x}\|_0 = |\{i | x_i \neq 0\}|$ \qquad $\|\mathbf{x}\|_2 = \sqrt{\sum_{i=1}^{N} \mathbf{x}_i^2} = \sqrt{\langle \mathbf{x}, \mathbf{x} \rangle}$\\
$\|\mathbf{x}\|_p = \left( \sum_{i=1}^{N} |x_i|^p \right)^{\frac{1}{p}}$\\
$\|\mathbf{M}\|_F =\allowbreak \sqrt{\sum_{i=1}^{m} \sum_{j=1}^{n}\mathbf{m}_{i,j}^2} =\allowbreak \sqrt{\sum_{i=1}^{\min\{m, n\}} \sigma_i^2} = \sqrt{trace(A^\top A)}$\\
$\|\mathbf{M}\|_1 = \sum_{i,j} | m_{i,j}|$ \qquad $\|\mathbf{M}\|_2 = \sigma_{\text{max}}(\mathbf{M})$\\
$\|\mathbf{M}\|_p = \max_{\mathbf{v} \neq 0} \frac{\|\mathbf{M}\mathbf{v}\|_p}{\|\mathbf{v}\|_p}$ \qquad $\|\mathbf{M}\|_\star = \sum_{i=1}^{\min(m, n)} \sigma_i$ \qquad $\|\mathbf{M}\|_G = \sqrt{\sum_{i,j} \mathbf{g}_{ij} \mathbf{m}_{ij}^2}$

\subsection*{Sums}
$\sum_{n=a}^b f(n) = \sum_{n=0}^b f(n) - \sum_{n=0}^{n-1} f(n)$\\
$\sum_{n=s}^{t} f(n)=\sum_{n=s+p}^{t+p}f(n-p)$\\
$\sum_{n\in B} f(n) = \sum_{m\in A} f(\sigma (m))$ for $\sigma : A\rightarrow B$ bij.\\
$\sum_{k\leq j \leq i \leq n}a_{ij} = \sum_{i=k}^n \sum_{j=k}^i a_{ij} = \sum_{j=0}^{n-k}\sum_{i=k}^{n-j} a_{i+j, i}$\\
$\sum_{i=s}^m \sum_{j=t}^n a_i c_j = (\sum_{i=s}^m a_i)(\sum_{j=t}^n c_j)$\\
$\sum_{i=1}^n i = n(n+1)/2$ \qquad $\sum_{i=1}^n 2i-1 = n^2$\\
$\sum_{i=0}^n log(i) = log(n!)$\qquad $\sum_{i=0}^{n-1} a^i=\frac{1-a^n}{1-a}$

\subsection*{Derivatives}
$\frac{\partial}{\partial \mathbf{x}}(\mathbf{b}^\top \mathbf{x}) = \frac{\partial}{\partial \mathbf{x}}(\mathbf{x}^\top \mathbf{b}) = \mathbf{b}$ \quad
$\frac{\partial}{\partial \mathbf{x}}(\mathbf{x}^\top \mathbf{x}) = 2\mathbf{x}$\\
$\frac{\partial}{\partial \mathbf{x}}(f(\mathbf{x})^\top\cdot g(\mathbf{x})) = f(\mathbf{x})^\top \frac{\partial g(\mathbf{x})}{\partial \mathbf{x}} + g(\mathbf{x})^\top \frac{\partial f(\mathbf{x})}{\partial \mathbf{x}}$\\
$\frac{\partial}{\partial \mathbf{x}}(\mathbf{x}^\top \mathbf{A}\mathbf{x}) = (\mathbf{A}^\top + \mathbf{A})\mathbf{x}$ \quad
$\frac{\partial}{\partial \mathbf{x}}(\mathbf{b}^\top \mathbf{A}\mathbf{x}) = \mathbf{A}^\top \mathbf{b}$\\
$\frac{\partial}{\partial \mathbf{X}}(\mathbf{c}^\top \mathbf{X} \mathbf{b}) = \mathbf{c}\mathbf{b}^\top$ \quad
$\frac{\partial}{\partial \mathbf{X}}(\mathbf{c}^\top \mathbf{X}^\top \mathbf{b}) = \mathbf{b}\mathbf{c}^\top$\\
$\frac{\partial}{\partial \mathbf{x}}(\| \mathbf{x}-\mathbf{b} \|_2) = \frac{\mathbf{x}-\mathbf{b}}{\|\mathbf{x}-\mathbf{b}\|_2}$ \quad
$\frac{\partial}{\partial \mathbf{x}}(\|\mathbf{x}\|^2_2) = \frac{\partial}{\partial \mathbf{x}} (\mathbf{x}^\top \mathbf{x}) = 2\mathbf{x}$\\
$\frac{\partial}{\partial \mathbf{X}}(\|\mathbf{X}\|_F^2) = 2\mathbf{X}$\quad
$\frac{\partial}{\partial \mathbf{X}} \mathbf{Tr}(\mathbf{X})=\mathbf{I}$ \\
$\frac{\partial}{\partial \mathbf{x}}(\|\mathbf{Ax - b}\|_2^2) = \mathbf{2(A^\top Ax-A^\top b)}$

\subsection*{Eigenvalue / -vectors}
Eigenvalue Problem: $\mathbf{Ax} = \lambda \mathbf{x}$\\
1. solve $\operatorname{det}(\mathbf{A} - \lambda \mathbf{I}) \overset{!}{=} 0$ resulting in $diag(\lambda_i)$\\
2. $\forall \lambda_i$:
solve $(\mathbf{A} - \lambda_i \mathbf{I}) \mathbf{x}_i = \mathbf{0}$, for $\mathbf{x}_i$.

\subsection*{Eigendecomposition}
$\mathbf{A} \in \mathbb{R}^{N \times N}$ then $\mathbf{A} = \mathbf{Q} \boldsymbol{\Lambda} \mathbf{Q}^{-1}$ with $\mathbf{Q} \in \mathbb{R}^{N \times N}$.\\
if fullrank: $\mathbf{A}^{-1} = \mathbf{Q} \boldsymbol{\Lambda}^{-1} \mathbf{Q}^{-1}$ and $(\boldsymbol{\Lambda}^{-1})_{i,i} = \frac{1}{\lambda_i}$.\\
if $\mathbf{A}$ symmetric: $A = \mathbf{Q} \boldsymbol{\Lambda} \mathbf{Q^\top}$ ($\mathbf{Q}$ orthogonal).

\subsection*{Probability / Statistics}
\begin{inparaitem}
	\item $P(x) := Pr[X = x] := \sum_{y \in Y} P(x, y)$
	\item $P(x|y) := Pr[X = x | Y = y] := \frac{P(x,y)}{P(y)},\quad \text{if } P(y) > 0$
	\item $\forall y \in Y: \sum_{x \in X} P(x|y) = 1$ (for any fixed $y$)
	\item Bayes: $P(x|y) = \frac{P(y|x)P(x)}{P(y)}$
	\item ($x_i$ partition) $\Rightarrow P(y) = \sum_{i=1}^n P(y|x_i)\cdot P(x_i)$
	\item $P(x|y) = P(x) \Leftrightarrow P(y|x) = P(y)$ (iff $X$, $Y$ ind.)
	\item $P(x_1, \ldots, x_n) = \prod_{i=1}^n P(x_i)$ (iff IID)
	\item $P(x \cup y)=P(x)+P(y)-P(x,y)$ (mut. excl: rm last term)
	\item $P(x)=\sum_i P(x,y_i)$
\end{inparaitem}